src/protocol/DNS.Protocol.Parser.EverParseAdapter.fst
@@ -20,6 +20,10 @@ let generated_dns_uncompressed_question_validator_linked : bool = true
 
 let generated_dns_uncompressed_question_answer_packet_validator_linked : bool = true
 
+let generated_dns_uncompressed_question_a_answer_packet_validator_linked : bool = true
+
+let generated_dns_uncompressed_question_aaaa_answer_packet_validator_linked : bool = true
+
 let generated_dns_header_validator = DNSProtocol.validate__dns_header
 
 let generated_dns_root_question_validator =
@@ -36,3 +40,9 @@ let generated_dns_uncompressed_question_validator qname_length =
 
 let generated_dns_uncompressed_question_answer_packet_validator qname_length rr_name_length rdata_length =
   DNSProtocol.validate__dns_uncompressed_question_answer_packet qname_length rr_name_length rdata_length
+
+let generated_dns_uncompressed_question_a_answer_packet_validator qname_length rr_name_length =
+  DNSProtocol.validate__dns_uncompressed_question_a_answer_packet qname_length rr_name_length
+
+let generated_dns_uncompressed_question_aaaa_answer_packet_validator qname_length rr_name_length =
+  DNSProtocol.validate__dns_uncompressed_question_aaaa_answer_packet qname_length rr_name_length
